\documentclass[pdflatex,ja=standard,a4paper]{bxjsarticle}
\usepackage{color}
\newcommand{\dif}{\mathrm{d}}
%opening
\title{正誤表}
\author{}

\begin{document}

\maketitle


\begin{enumerate}
\item[p.35 練習問題２]\quad 
\begin{description}
\item[誤：] 
\begin{eqnarray*}
\left{\max\left\{\frac{1200+800}{2}-750,0\right\}\\
	\max\left\{\frac{1000+500}{2}-750,0\right\}\\
	\max\left\{\frac{1200+800}{2}-750,0\right\}
\right)
=\left(
250 \\ 0 \\ 0
\right)
\end{eqnarray*}
\item[正：] 
\begin{eqnarray*}
			\lim_{n\to\infty}(\sqrt{n+2}-\sqrt{n})
			&=& \lim_{n\to\infty}
			\frac{(\sqrt{n+2}-\sqrt{n})(\sqrt{n+2}+\sqrt{n})}{\sqrt{n+2}+\sqrt{n}}\\
		&=& \lim_{n\to\infty}
		\frac{2}{(\sqrt{n+\textcolor{red}{2}}+\sqrt{n})}=0.
\end{eqnarray*}
\end{description}
\item[p.114 l.9]\quad 
\begin{description}
\item[誤：] 
ここで，$x\to a+$とすると，${\displaystyle\lim_{x\to a}f(x)=\lim_{x\to a}\textcolor{red}{f}(x)=\infty}$であること
\item[正：] 
ここで，$x\to a+$とすると，${\displaystyle\lim_{x\to a}f(x)=\lim_{x\to a}\textcolor{red}{g}(x)=\infty}$であること
\end{description}
\item[p.143 l.10]
\item[誤：] 
$$F=f(x_1+h_1,x_2+h_2)-f(x_1+h_1,x_2)-f(x_1,x_2+h_2)\textcolor{red}{-}f(x_1,x_2)$$
\item[正：] 
$$F=f(x_1+h_1,x_2+h_2)-f(x_1+h_1,x_2)-f(x_1,x_2+h_2)\textcolor{red}{+}f(x_1,x_2)$$

\item[p.148 l.4]
\item[誤：] 
$$dy=\frac{\partial f}{\partial x_1}\dif x_1+\frac{\partial f}{\partial x_2}\dif x_2=
\frac{x_2^2}{(x_{\textcolor{red}{2}}^{\textcolor{red}{2}}+x_2)^2}\dif x_1+
\frac{x_1^2}{(x_1^{\textcolor{red}{2}}+x_2)^2}\dif x_2.$$
\item[正：] 
$$dy=\frac{\partial f}{\partial x_1}\dif x_1+\frac{\partial f}{\partial x_2}\dif x_2
2=
\frac{x_2^2}{(x_{\textcolor{red}{1}}+x_2)^2}\dif x_1+
\frac{x_1^2}{(x_1+x_2)^2}\dif x_2.$$
\item[p.149 l.8]
\item[誤：] 
$$\lim_{\Delta t\to0}
\left\{
\frac{\phi(t+\Delta t),\psi(t+\Delta t)-f(\phi(t),\psi(t))}{\Delta t}-f_{x_1}\frac{\Delta x_1}{\Delta t}-f_{x_2}\frac{\Delta x_2}{\Delta t}
\right\}=0$$
\item[正：] 
$$\lim_{\Delta t\to0}
\left\{
\frac{\textcolor{red}{f(}\phi(t+\Delta t),\psi(t+\Delta t)-f(\phi(t),\psi(t))}{\Delta t}-f_{x_1}\frac{\Delta x_1}{\Delta t}-f_{x_2}\frac{\Delta x_2}{\Delta t}
\right\}=0$$
\end{enumerate}
\end{document}
